tests/Calls.v
@@ -1,0 +1,40 @@
+(* All low addresses use ordinary account dispatch; native precompiles are absent. *)
+From Stdlib Require Import List ZArith.
+From EVMOpSem Require Import Lem.coqharness block.
+Import ListNotations.
+Local Open Scope Z_scope.
+Set Default Goal Selector "!".
+
+Definition low_call : call_arguments :=
+  {| callarg_gas := word256FromNumeral 0; callarg_code := word160FromNumeral 1;
+     callarg_recipient := word160FromNumeral 1; callarg_value := word256FromNumeral 0;
+     callarg_data := []; callarg_output_begin := word256FromNumeral 0;
+     callarg_output_size := word256FromNumeral 0 |}.
+
+Theorem low_call_dispatches g v area :
+  @eq _ (g_vmstate g) (InstructionToEnvironment (ContractCall low_call) v area) ->
+  exists h, @eq _ (step Homestead (Continue g)) (Continue h).
+Proof.
+  intro Hr. unfold step. rewrite Hr.
+  destruct (word256ULT _ _ || nat_gtb _ _); eexists; reflexivity.
+Qed.
+
+Theorem low_call_enters_ordinary_code g v area :
+  @eq _ (g_vmstate g) (InstructionToEnvironment (ContractCall low_call) v area) ->
+  @eq _ (word256ULT
+    (block_account_balance (update_return (g_current g) (cctx_this (g_cctx g)) v
+      (cctx_this (g_cctx g)))) (callarg_value low_call) ||
+      nat_gtb (List.length (g_stack g)) 1023) false ->
+  exists h, @eq _ (step Homestead (Continue g)) (Continue h) /\
+    @eq _ (cctx_this (g_cctx h)) (word160FromNumeral 1) /\
+    @eq _ (cctx_program (g_cctx h))
+      (block_account_code (update_call
+        (update_return (g_current g) (cctx_this (g_cctx g)) v)
+        (cctx_this (g_cctx g)) low_call (word160FromNumeral 1))).
+Proof.
+  intros Hr Hallowed. unfold step. rewrite Hr, Hallowed.
+  eexists. repeat split; reflexivity.
+Qed.
+
+
+Print Assumptions low_call_enters_ordinary_code.
